remove tree sections

new/copy.v
@@ -3,83 +3,79 @@ Require Import Program.Equality.
 Require Import Omega.
 Require Import Arith Arith.Even Arith.Div2.
 
-Section copy.
-  Variable A : Set.
-  Variable x : A.
+Inductive Copy2R : A -> nat -> bin_tree * bin_tree -> nat -> Prop :=
+  C2R_zero :
+    forall x,
+      Copy2R x 0 (bt_node x bt_mt bt_mt, bt_mt) 1
+| C2R_even :
+    forall x m time s t,
+      Copy2R x m (s,t) time ->
+      Copy2R x (2*m+1) (bt_node x s t, bt_node x t t) (time+2)
+| C2R_odd :
+    forall x m time s t,
+      Copy2R x m (s,t) time ->
+      Copy2R x (2*m+2) (bt_node x s s, bt_node x s t) (time+2).
+Hint Constructors Copy2R.
 
-  Inductive Copy2R : nat -> (bin_tree A) * (bin_tree A) -> nat -> Prop :=
-    C2R_zero : 
-      Copy2R 0 (bt_node x (bt_mt A) (bt_mt A),bt_mt A) 1
-  | C2R_even : 
-      forall m time s t, 
-        Copy2R m (s,t) time ->
-        Copy2R (2*m+1) (bt_node x s t, bt_node x t t) (time+2)
-  | C2R_odd : 
-      forall m time s t, 
-        Copy2R m (s,t) time ->
-        Copy2R (2*m+2) (bt_node x s s, bt_node x s t) (time+2).
-  Hint Constructors Copy2R.
+Inductive CopyR : A -> nat -> bin_tree -> nat -> Prop :=
+  CR :
+    forall x n bt1 bt2 time,
+      Copy2R x n (bt1,bt2) time ->
+      CopyR x n bt2 time.
+Hint Constructors CopyR.
 
-  Inductive CopyR : nat -> bin_tree A -> nat -> Prop :=
-    CR : 
-      forall n bt1 bt2 time,
-        Copy2R n (bt1,bt2) time ->
-        CopyR n bt2 time.
-  Hint Constructors CopyR.
+Lemma copy2 :
+  forall x (n:nat),
+    {pr | exists time, Copy2R x n pr time}.
+Proof.
+  intros x.
+  apply (well_founded_induction_type
+           lt_wf
+           (fun n => {pr | exists time, Copy2R x n pr time})).
+  intros n IND.
+  destruct n.
+  eauto.
 
-  Lemma copy2 : 
-    forall (n:nat),
-      {pr | exists time, Copy2R n pr time}.
-  Proof.
-    apply (well_founded_induction_type
-             lt_wf
-             (fun n => {pr | exists time, Copy2R n pr time})).
-    intros n IND.
-    destruct n.
-    eauto.
+  destruct (IND (div2 n)) as [PR IND2];[auto|].
+  clear IND; destruct PR as [s t].
+  destruct (even_odd_dec n).
 
-    destruct (IND (div2 n)) as [PR IND2];[auto|].
-    clear IND; destruct PR as [s t].
-    destruct (even_odd_dec n).
+  exists (bt_node x s t, bt_node x t t).
+  destruct IND2.
+  exists (x0+2).
+  replace (S n) with (2*(div2 n)+1).
+  eauto.
+  rewrite (even_double n) at 2;[|assumption].
+  unfold double.
+  omega.
 
-    exists (bt_node x s t, bt_node x t t).
-    destruct IND2.
-    exists (x0+2).
-    replace (S n) with (2*(div2 n)+1).
-    eauto.
-    rewrite (even_double n) at 2;[|assumption].
-    unfold double.
-    omega.
+  exists (bt_node x s s, bt_node x s t).
+  destruct IND2.
+  exists (x0+2).
+  replace (S n) with (2*(div2 n)+2).
+  eauto.
+  rewrite (odd_double n) at 2;[|assumption].
+  unfold double.
+  omega.
 
-    exists (bt_node x s s, bt_node x s t).
-    destruct IND2.
-    exists (x0+2).
-    replace (S n) with (2*(div2 n)+2).
-    eauto.
-    rewrite (odd_double n) at 2;[|assumption].
-    unfold double.
-    omega.
+Defined.
 
-  Defined.
-
-  Theorem copy : 
-    forall (n:nat), {bt | exists time, CopyR n bt time}.
-  Proof.
-    intros n.
-    destruct (copy2 n) as [[s t] E].
-    exists t.
-    destruct E.
-    eauto.
-  Defined.
-
-End copy.
+Theorem copy :
+  forall x (n:nat), {bt | exists time, CopyR x n bt time}.
+Proof.
+  intros x n.
+  destruct (copy2 x n) as [[s t] E].
+  exists t.
+  destruct E.
+  eauto.
+Defined.
 
 Lemma Copy2_produces_Braun :
-  forall A x n bt1 bt2 time, 
-    (Copy2R A x n (bt1,bt2) time)
+  forall x n bt1 bt2 time,
+    (Copy2R x n (bt1,bt2) time)
     -> Braun bt1 (n+1) /\ Braun bt2 n.
 Proof.
-  intros A x n s t time CSR.
+  intros x n s t time CSR.
   dependent induction CSR; try (inversion IHCSR; clear IHCSR).
 
   constructor.
@@ -104,39 +100,39 @@ Proof.
   constructor;[omega|assumption|assumption].
 Qed.
 
-Lemma Copy_produces_Braun : 
-  forall A x n bt time, 
-    (CopyR A x n bt time) ->
+Lemma Copy_produces_Braun :
+  forall x n bt time,
+    (CopyR x n bt time) ->
     Braun bt n.
 Proof.
-  intros A x n bt time CSR.
+  intros x n bt time CSR.
   inversion CSR.
   apply Copy2_produces_Braun in H.
   inversion H.
   assumption.
 Qed.
 
-Lemma Copy2R_running_time : 
-  forall A x n bt1 bt2 time, 
-    Copy2R A x n (bt1,bt2) time ->
+Lemma Copy2R_running_time :
+  forall x n bt1 bt2 time,
+    Copy2R x n (bt1,bt2) time ->
     time = ((2 * fl_log n) + 1).
 Proof.
-  intros A x n bt1 bt2 time Copy2.
+  intros x n bt1 bt2 time Copy2.
   dependent induction Copy2.
   compute; reflexivity.
 
   replace (2*m+1) with (m+m+1); [|omega].
   rewrite fl_log_odd.
   omega.
-  
+
   replace (2*m+2) with ((m+1)+(m+1));[|omega].
   rewrite fl_log_even.
   omega.
 Qed.
 
-Lemma CopyR_running_time : 
-  forall A x n bt1 time, 
-    CopyR A x n bt1 time ->
+Lemma CopyR_running_time :
+  forall x n bt1 time,
+    CopyR x n bt1 time ->
     time = ((2 * fl_log n) + 1).
   intros.
   inversion H.
