new/braun.v
@@ -1,22 +1,19 @@
 Set Implicit Arguments.
 
-Section braun.
-  Variable A : Set.
+Variable A : Set.
 
-  Inductive bin_tree : Set :=
-  | bt_mt : bin_tree
-  | bt_node : A -> bin_tree -> bin_tree -> bin_tree.
-  Hint Constructors bin_tree.
-  
-  Inductive Braun : bin_tree -> nat -> Prop :=
-  | B_mt :
-      Braun bt_mt 0
-  | B_node :
-      forall (x:A) s s_size t t_size,
-        t_size <= s_size <= t_size+1 ->
-        Braun s s_size ->
-        Braun t t_size ->
-        Braun (bt_node x s t) (s_size+t_size+1).
-  Hint Constructors Braun.
-  
-End braun.
+Inductive bin_tree : Set :=
+| bt_mt : bin_tree
+| bt_node : A -> bin_tree -> bin_tree -> bin_tree.
+Hint Constructors bin_tree.
+
+Inductive Braun : bin_tree -> nat -> Prop :=
+| B_mt :
+    Braun bt_mt 0
+| B_node :
+    forall (x:A) s s_size t t_size,
+      t_size <= s_size <= t_size+1 ->
+      Braun s s_size ->
+      Braun t t_size ->
+      Braun (bt_node x s t) (s_size+t_size+1).
+Hint Constructors Braun.
