new/make_array_linear.v
@@ -3,108 +3,103 @@ Require Import Arith Arith.Even Arith.Div2 List.
 Require Import Program.
 Require Import Omega.
 
-Section array.
-  Variable A : Set.
+Inductive MakeArrayLinearR : list A -> bin_tree -> nat -> Prop :=
+| MALR_zero :
+    MakeArrayLinearR nil bt_mt 0
+| MALR_succ :
+    forall x xs bt bt' time insert_time,
+      InsertR x bt bt' insert_time ->
+      MakeArrayLinearR        xs bt                  time ->
+      MakeArrayLinearR (x :: xs) bt' (time + insert_time).
+Hint Constructors MakeArrayLinearR.
 
-  Inductive MakeArrayLinearR : list A -> bin_tree A -> nat -> Prop :=
-  | MALR_zero : 
-      MakeArrayLinearR nil (bt_mt A) 0
-  | MALR_succ :
-      forall x xs bt bt' time insert_time,
-        InsertR A x bt bt' insert_time ->
-        MakeArrayLinearR        xs bt                  time ->
-        MakeArrayLinearR (x :: xs) bt' (time + insert_time).
-  Hint Constructors MakeArrayLinearR.
+Theorem MakeArrayLinearR_SequenceR :
+  forall xs bt n,
+    MakeArrayLinearR xs bt n ->
+    SequenceR bt xs.
+Proof.
+  intros xs bt n MALR.
+  induction MALR; eauto.
+  eapply InsertR_SequenceR; eauto.
+Qed.
 
-  Theorem MakeArrayLinearR_SequenceR :
-    forall xs bt n,
-      MakeArrayLinearR xs bt n ->
-      SequenceR A bt xs.
-  Proof.
-    intros xs bt n MALR.
-    induction MALR; eauto.
-    apply SR_mt.
-    eapply InsertR_SequenceR; eauto.
-  Qed.
+Theorem make_array_linear :
+  forall xs,
+    { bt | exists n, MakeArrayLinearR xs bt n }.
+Proof.
+  induction xs as [| x xs]; [eauto |].
+  destruct IHxs as [bt IR].
+  remember (insert x bt).
+  clear Heqs.
+  destruct s as [bt' insIR'].
+  exists bt'.
+  destruct IR as [indTime indR].
+  destruct insIR' as [insTime insIR].
+  exists (indTime + insTime).
+  apply (MALR_succ _ _ bt); eauto.
+Defined.
 
-  Theorem make_array_linear :
-    forall xs,
-      { bt | exists n, MakeArrayLinearR xs bt n }.
-  Proof.
-    induction xs as [| x xs]; [eauto |].
-    destruct IHxs as [bt IR].
-    remember (insert A x bt).
-    clear Heqs.
-    destruct s as [bt' insIR'].
-    exists bt'.
-    destruct IR as [indTime indR].
-    destruct insIR' as [insTime insIR].
-    exists (indTime + insTime).
-    apply (MALR_succ _ _ bt); eauto.
-  Defined.
-  
-  Theorem MakeArrayLinearR_Braun :
-    forall xs bt n,
-      MakeArrayLinearR xs bt n ->
-      Braun bt (length xs).
-  Proof.
-    intro xs.
-    induction xs as [| x xs]; intros bt n MkArrR.
+Theorem MakeArrayLinearR_Braun :
+  forall xs bt n,
+    MakeArrayLinearR xs bt n ->
+    Braun bt (length xs).
+Proof.
+  intro xs.
+  induction xs as [| x xs]; intros bt n MkArrR.
 
-    simpl.
-    inversion_clear MkArrR.
-    constructor.
+  simpl.
+  inversion_clear MkArrR.
+  constructor.
 
-    simpl.
-    inversion_clear MkArrR.
-    apply (InsertR_Braun A x (length xs) insert_time bt0).
-    apply (IHxs bt0 time H0).
-    assumption.
-  Qed.
+  simpl.
+  inversion_clear MkArrR.
+  apply (InsertR_Braun x (length xs) insert_time bt0).
+  apply (IHxs bt0 time H0).
+  assumption.
+Qed.
 
-  Theorem MakeArrayLinearR_correct :
-    forall xs bt n,
-      MakeArrayLinearR xs bt n ->
-      forall i x,
-        IndexR A bt i x ->
-        ListIndexR A xs i x.
-  Proof.
-    intros xs bt n MALR i x IR.
-    eapply SequenceR_IndexR.
-    apply IR.
-    eapply MakeArrayLinearR_Braun.
-    apply MALR.
-    eapply MakeArrayLinearR_SequenceR.
-    apply MALR.
-  Qed.
+Theorem MakeArrayLinearR_correct :
+  forall xs bt n,
+    MakeArrayLinearR xs bt n ->
+    forall i x,
+      IndexR bt i x ->
+      ListIndexR A xs i x.
+Proof.
+  intros xs bt n MALR i x IR.
+  eapply SequenceR_IndexR.
+  apply IR.
+  eapply MakeArrayLinearR_Braun.
+  apply MALR.
+  eapply MakeArrayLinearR_SequenceR.
+  apply MALR.
+Qed.
 
-  Fixpoint rt_naive n : nat :=
-    match n with
-      | 0 => 0
-      | S n' => rt_naive n' + (fl_log n' + 1)
-    end.
+Fixpoint rt_naive n : nat :=
+  match n with
+    | 0 => 0
+    | S n' => rt_naive n' + (fl_log n' + 1)
+  end.
 
-  Example rt_naive_ex :
-    map rt_naive (1 :: 2 :: 3 :: 4 ::  5 ::  6 ::  7 ::  8 ::  9 :: 10 :: nil)
-               = (1 :: 3 :: 5 :: 8 :: 11 :: 14 :: 17 :: 21 :: 25 :: 29 :: nil).
-  Proof.
-    auto.
-  Qed.
+Example rt_naive_ex :
+  map rt_naive (1 :: 2 :: 3 :: 4 ::  5 ::  6 ::  7 ::  8 ::  9 :: 10 :: nil)
+  = (1 :: 3 :: 5 :: 8 :: 11 :: 14 :: 17 :: 21 :: 25 :: 29 :: nil).
+Proof.
+  auto.
+Qed.
 
-  Theorem MakeArrayLinearR_time :
-    forall xs bt t,
-      MakeArrayLinearR xs bt t ->
-      t = rt_naive (length xs).
-  Proof.
-    intros xs bt t MALR.
-    induction MALR.
-    auto.
-    rename H into IR.
-    subst.
-    apply MakeArrayLinearR_Braun in MALR.
-    eapply (InsertR_time _ _ _ _ _ _ MALR) in IR.
-    subst.
-    simpl.
-    auto.
-  Qed.  
-End array.
+Theorem MakeArrayLinearR_time :
+  forall xs bt t,
+    MakeArrayLinearR xs bt t ->
+    t = rt_naive (length xs).
+Proof.
+  intros xs bt t MALR.
+  induction MALR.
+  auto.
+  rename H into IR.
+  subst.
+  apply MakeArrayLinearR_Braun in MALR.
+  eapply (InsertR_time _ _ _ _ _ MALR) in IR.
+  subst.
+  simpl.
+  auto.
+Qed.
