new/same_structure.v
@@ -5,57 +5,53 @@ Require Import braun util Omega.
 Require Import Program.Equality.
 Set Implicit Arguments.
 
-Module same_structure.
-  Variable A : Set.
+Inductive same_structure : bin_tree -> bin_tree -> Prop :=
+| SS_mt :
+    same_structure bt_mt bt_mt
+| SS_node :
+    forall (x1 x2 : A) l1 l2 r1 r2,
+      same_structure l1 l2 ->
+      same_structure r1 r2 ->
+      same_structure (bt_node x1 l1 r1)
+                     (bt_node x2 l2 r2).
+Hint Constructors same_structure.
 
-  Inductive same_structure : bin_tree A -> bin_tree A -> Prop :=
-    | SS_mt :
-        same_structure (bt_mt A) (bt_mt A)
-    | SS_node :
-        forall (x1 x2 : A) l1 l2 r1 r2,
-          same_structure l1 l2 ->
-          same_structure r1 r2 ->
-          same_structure (bt_node x1 l1 r1)
-                         (bt_node x2 l2 r2).
-  Hint Constructors same_structure.
+Theorem same_structure_same_size :
+  forall bt1 bt2,
+    same_structure bt1 bt2 ->
+    forall n1 n2,
+      Braun bt1 n1 ->
+      Braun bt2 n2 ->
+      n1 = n2.
+Proof.
+  intros bt1 bt2 SS.
+  induction SS; intros n1 n2 B1 B2;
+  inversion_clear B1;
+  inversion_clear B2; eauto.
+Qed.
 
-  Theorem same_structure_same_size : 
-    forall bt1 bt2,
-      same_structure bt1 bt2 ->
-      forall n1 n2,
-        Braun bt1 n1 ->
-        Braun bt2 n2 ->
-        n1 = n2.
-  Proof.
-    intros bt1 bt2 SS.
-    induction SS; intros n1 n2 B1 B2;
-    inversion_clear B1;
-    inversion_clear B2; eauto.
-  Qed.
+Theorem same_size_same_structure :
+  forall n bt1 bt2,
+    Braun bt1 n ->
+    Braun bt2 n ->
+    same_structure bt1 bt2.
+Proof.
+  apply (well_founded_ind
+           lt_wf
+           (fun n => forall (b1 b2 : bin_tree),
+                       Braun b1 n -> Braun b2 n -> same_structure b1 b2)).
+  intros n IH bt1 bt2 B1 B2.
+  dependent destruction bt1; dependent destruction bt2; eauto;
+  inversion B1; subst;
+  inversion B2; subst; eauto.
 
-  Theorem same_size_same_structure :
-    forall n bt1 bt2,
-      Braun bt1 n ->
-      Braun bt2 n ->
-      same_structure bt1 bt2.
-  Proof.
-    apply (well_founded_ind 
-             lt_wf 
-             (fun n => forall (b1 b2 : bin_tree A), 
-                         Braun b1 n -> Braun b2 n -> same_structure b1 b2)).
-    intros n IH bt1 bt2 B1 B2.
-    dependent destruction bt1; dependent destruction bt2; eauto;
-    inversion B1; subst;
-    inversion B2; subst; eauto.
+  apply plusone_ne_zero in H2; inversion H2.
+  symmetry in H. apply plusone_ne_zero in H; inversion H.
+  assert (s_size = s_size0); try omega.
+  assert (t_size = t_size0); try omega.
+  subst.
 
-    apply plusone_ne_zero in H2; inversion H2.
-    symmetry in H. apply plusone_ne_zero in H; inversion H.
-    assert (s_size = s_size0); try omega.
-    assert (t_size = t_size0); try omega.
-    subst.
-
-    eapply SS_node.
-    eapply IH; eauto; omega.
-    eapply IH; eauto; omega.
-  Qed.  
-End same_structure.
+  eapply SS_node.
+  eapply IH; eauto; omega.
+  eapply IH; eauto; omega.
+Qed.
